theories/soundness/priv_call.v
@@ -1,0 +1,388 @@
+(*
+ * Copyright (c) Meta Platforms, Inc. and affiliates.
+ *
+ * This source code is licensed under the MIT license found in the
+ * LICENSE file in the root directory of this source tree.
+ *)
+From stdpp Require Import base strings gmap stringmap fin_maps.
+From iris.base_logic Require Import upred derived.
+From iris.base_logic.lib Require Import iprop own.
+From iris.algebra Require Import ofe cmra gmap_view.
+From iris.proofmode Require Import tactics.
+
+From shack Require Import lang progdef subtype typing eval heap modality interp.
+From shack.soundness Require Import expr defs.
+
+Section proofs.
+  (* assume a given set of class definitions *)
+  Context `{PDC: ProgDefContext}.
+  (* assume some SDT constraints and their properties *)
+  Context `{SDTCS: SDTClassSpec}.
+
+  (* Helping the inference with this notation that hides pdefs *)
+  Local Notation "Δ ⊢ s <: t" := (@subtype _ _ Δ Plain s t) (at level 70, s at next level, no associativity).
+  Local Notation "Δ ⊢ s <D: t" := (@subtype _ _ Δ Aware s t) (at level 70, s at next level, no associativity).
+
+  (* Iris semantic context *)
+  Context `{!sem_heapGS Θ}.
+
+  (* TODO: keep in sync with call_soundness. Ideally, factor as much as
+   * possible and refactor.
+   *)
+  Lemma priv_call_soundness C Δ kd rigid Γ lhs t σ name mdef args:
+    wf_cdefs pdefs →
+    wf_lty Γ →
+    Forall wf_constraint Δ →
+    Forall (bounded_constraint rigid) Δ →
+    ok_ty Δ (this_type Γ) →
+    type_of_this Γ = (t, σ) →
+    has_method name t C mdef →
+    mdef.(methodvisibility) = Private →
+    dom (methodargs mdef) = dom args →
+    (∀ (x : string) (ty : lang_ty) (arg : expr),
+       methodargs mdef !! x = Some ty →
+       args !! x = Some arg →
+       expr_has_ty Δ Γ rigid kd arg (subst_ty σ ty)) →
+    ∀ Σ st st' n,
+    length Σ = rigid →
+    cmd_eval C st (CallC lhs ThisE name args) st' n →
+    □ interp_env_as_mixed Σ -∗
+    □ Σinterp Σ Δ -∗
+    □ (▷ (∀ (a : tag) (a0 : list constraint) (a1 : subtype_kind)
+            (a2 : nat) (a3 : local_tys) (a4 : cmd)
+            (a5 : local_tys),
+            ⌜wf_lty a3⌝ -∗
+            ⌜bounded_lty a2 a3⌝ -∗
+            ⌜ok_ty a0 (this_type a3)⌝ -∗
+            ⌜Forall wf_constraint a0⌝ -∗
+            ⌜Forall (bounded_constraint a2) a0⌝ -∗
+            ∀ (_ : cmd_has_ty a a0 a1 a2 a3 a4 a5)
+              (x0 : list (interp Θ)) (x1 x2 : local_env * heap)
+              (x3 : nat) (_ : length x0 = a2) (_ : cmd_eval a x1 a4 x2 x3),
+              □ interp_env_as_mixed x0 -∗
+              □ Σinterp x0 a0 -∗
+              heap_models x1.2 ∗ interp_local_tys x0 a3 x1.1 -∗
+              |=▷^x3 heap_models x2.2 ∗ interp_local_tys x0 a5 x2.1)) -∗
+    heap_models st.2 ∗ interp_local_tys Σ Γ st.1 -∗
+    |=▷^n heap_models st'.2 ∗
+          interp_local_tys Σ (<[lhs:=subst_ty σ (methodrettype mdef)]> Γ) st'.1.
+  Proof.
+    move => wfpdefs wflty hΔ hΔb hokthis ht hhasm hpriv hdom hi Σ st st' n hrigid hc.
+    iIntros "#hΣ #hΣΔ #IH".
+    inv hc; simpl.
+    assert (wfpdefs0 := wfpdefs).
+    destruct wfpdefs0.
+    iIntros "[Hh #Hle]".
+    (* make the script more resilient. Should provide a proper inversion
+     * lemma but this is the next best thing.
+     *)
+    rename H3 into heval_recv.
+    rename H4 into hmap.
+    rename H5 into hheap.
+    rename H6 into hhasm0.
+    rename H9 into hmdom.
+    rename H13 into heval_body.
+    rename H14 into heval_ret.
+    assert (ht0: this_type Γ = ClassT t σ).
+    { destruct Γ as [[] Γ].
+      rewrite /this_type /type_of_this /= in ht.
+      rewrite /this_type /type_of_this /=.
+      by injection ht; intros; subst; clear ht.
+    }
+    assert (hwfthis : wf_ty (ClassT t σ)).
+    { rewrite -ht0.
+      by apply wflty.
+    }
+    assert (hwfσ : Forall wf_ty σ) by by apply wf_ty_class_inv in hwfthis.
+    assert (hcdef : ∃ cdef, pdefs !! C = Some cdef).
+    { apply has_method_from_def in hhasm => //.
+      destruct hhasm as (cdef & _ & hcdef & _).
+      by exists cdef.
+    }
+    destruct hcdef as [cdef hcdef].
+    assert (hrecv: expr_has_ty Δ Γ (length Σ) kd ThisE (ClassT t σ)).
+    { rewrite -ht0.
+      by apply ThisTy.
+    }
+    (* Get inherits relation between dynamic tag and static tag *)
+    iDestruct (expr_soundness Δ (length Σ) Σ _ ThisE with "hΣ hΣΔ Hle") as "#Hrecv" => //.
+    rewrite interp_class_unfold //.
+    iDestruct "Hrecv" as (? t1 def def1 σin Σt fields ifields) "[%Hpure [_ [_ [_ [_ Hl]]]]]".
+    destruct Hpure as ([= <-] & hdef & hdef1 & hlen & ? & hin_t1_t & hfields & hidom).
+    iDestruct "Hh" as (sh) "(H● & %Hdom & #Hh)".
+    iDestruct (sem_heap_own_valid_2 with "H● Hl") as "#HΦ".
+    iDestruct ("Hh" with "[//]") as (?) "[H H▷]".
+    iRewrite "H" in "HΦ".
+    rewrite option_equivI prod_equivI /=.
+    iDestruct "HΦ" as "[%Ht HΦ]".
+    fold_leibniz; subst.
+    destruct (has_method_ordered _ _ _ _ _ _ _ _ wf_override wf_parent
+      wf_constraints_bounded wf_methods_bounded hin_t1_t hhasm0 hhasm)
+    as (odef0 & odef & σt1_o0 & σt_o & omdef0 & omdef & hodef0 & hodef & homdef0 & homdef & hin_t1_o0
+    & hin_t_o & -> & -> & (*hpub0 &*) hincl0 & [hh | hh]); last first.
+    (* TODO: update this when proper private methods are implemented *)
+    { destruct hh as (σ_ & hin_ & _).
+      assert (hin__: inherits_using orig C (subst_ty σ_ <$> σt_o)).
+      { by eapply inherits_using_trans. }
+      move: (wf_override _ _ _ _ _ _ _ _ hodef0 hodef hin__  homdef0 homdef).
+      rewrite hpriv.
+      by intro hf; elim hf.
+    }
+    destruct hh as (_ & -> & -> & <-); simplify_eq.
+    (* END TODO *)
+    assert (hh: Forall wf_ty σt_o ∧ length cdef.(generics) = length σt_o).
+    { apply inherits_using_wf in hin_t_o => //.
+      destruct hin_t_o as (?&?&?&hh).
+      split; first by apply wf_ty_class_inv in hh.
+      inv hh; by simplify_eq.
+    }
+    destruct hh as [hFσt_o heq1].
+    assert (hokc: ok_ty cdef.(constraints) (ClassT C (gen_targs (length cdef.(generics))))).
+    { econstructor => //.
+      - move => k ty hty.
+        apply lookup_gen_targs in hty as ->.
+        by constructor.
+      - move => k [c0 c1] hc /=.
+        rewrite !subst_ty_id.
+        + apply SubConstraint.
+          by apply elem_of_list_lookup_2 in hc.
+        + apply wf_constraints_bounded in hcdef.
+          rewrite /wf_cdef_constraints_bounded Forall_lookup in hcdef.
+          by apply hcdef in hc as [].
+        + apply wf_constraints_bounded in hcdef.
+          rewrite /wf_cdef_constraints_bounded Forall_lookup in hcdef.
+          by apply hcdef in hc as [].
+    }
+    assert (hF: Forall (bounded (length σ)) σt_o).
+    { apply inherits_using_wf in hin_t_o => //.
+      destruct hin_t_o as (? & ? & ? & ?); simplify_eq.
+      inv hwfthis; simplify_eq.
+      by rewrite H5.
+    }
+    assert (hh: wf_mdef_ty C cdef.(constraints) (length cdef.(generics)) (gen_targs (length cdef.(generics))) omdef).
+    { apply wf_mdefs in hcdef.
+      by apply hcdef in homdef0.
+    }
+    destruct hh as (Γ' & hwfΓ' & hbody & hret).
+    assert (hwf_lty0 : wf_lty
+    {|
+      type_of_this := (C, gen_targs (length cdef.(generics)));
+      ctxt := methodargs omdef
+    |}).
+    { split.
+      - rewrite /this_type /=.
+        eapply wf_ty_class => //; first by rewrite length_gen_targs.
+        by apply gen_targs_wf_2.
+      - rewrite map_Forall_lookup => k tk hk.
+        apply wf_methods_wf in hcdef.
+        apply hcdef in homdef0.
+        by apply homdef0 in hk.
+    }
+    assert (hbounded : bounded_lty (length cdef.(generics))
+    {|
+      type_of_this := (C, gen_targs (length cdef.(generics)));
+      ctxt := methodargs omdef
+    |}).
+    { split => /=.
+      - rewrite /this_type /=.
+        constructor.
+        by apply bounded_gen_targs.
+      - rewrite map_Forall_lookup => k tk hk.
+        apply wf_methods_bounded in hcdef.
+        apply hcdef in homdef0.
+        by apply homdef0 in hk.
+    }
+    assert (hΔ1 : Forall wf_constraint def1.(constraints)).
+    { by apply wf_constraints_wf in hdef1.  }
+    apply cmd_eval_subst in heval_body.
+    rewrite expr_eval_subst in heval_ret.
+    iModIntro; iNext.
+    iAssert (□ interp_env_as_mixed (interp_list Σ (subst_ty σ <$> σt_o)))%I as "#hΣc".
+    { iModIntro.
+      iIntros (k ϕ hk v) "hv".
+      apply list_lookup_fmap_inv in hk as [ty0 [-> h0]].
+      apply list_lookup_fmap_inv in h0 as [ty1 [-> h1]].
+      iDestruct (submixed_is_inclusion_aux with "hΣ hv") as "hh".
+      - apply wf_ty_subst => //.
+        rewrite Forall_lookup in hFσt_o; by eapply hFσt_o.
+      - by rewrite interp_mixed_unfold.
+    }
+    assert (hokt: ok_ty Δ (ClassT t σ)).
+    { destruct Γ as [[] ?].
+      rewrite /this_type /= in ht, hokthis.
+      injection ht; intros; subst; clear ht.
+      done.
+    }
+    assert (hok0: ok_ty (Δ ++ subst_constraints σ (constraints def)) (ClassT C (subst_ty σ <$> σt_o))).
+    { econstructor => //.
+      - move => k ty hk.
+        apply list_lookup_fmap_inv in hk as [ty0 [-> h0]].
+        eapply ok_ty_subst => //.
+        + apply inherits_using_ok in hin_t_o => //.
+          destruct hin_t_o as (tdef & htdef & hokC); simplify_eq.
+          inv hokC.
+          by apply H2 in h0.
+        + rewrite Forall_lookup in hFσt_o; by eapply hFσt_o.
+        + inv hokt.
+          apply Forall_lookup => ? ty hl.
+          by apply H2 in hl.
+      - move => k [c0 c1] hc /=.
+        assert (h0 := hcdef).
+        apply wf_constraints_bounded in h0.
+        rewrite /wf_cdef_constraints_bounded Forall_lookup in h0.
+        rewrite -!subst_ty_subst.
+        + apply subtype_weaken with (Δ := subst_constraints σ def.(constraints)); last by set_solver.
+          apply subtype_subst => //.
+          apply inherits_using_ok in hin_t_o => //.
+          destruct hin_t_o as (tdef & htdef & hokC); simplify_eq.
+          inv hokC; simplify_eq.
+          by apply H4 in hc.
+        + rewrite -heq1; by apply h0 in hc as [].
+        + rewrite -heq1; by apply h0 in hc as [].
+    }
+    assert (hok0_: ok_ty Δ (ClassT C (subst_ty σ <$> σt_o))).
+    { eapply ok_ty_constraint_trans with (kd := Aware); first by apply hok0.
+      move => k c hc /=.
+      rewrite lookup_app in hc.
+      destruct (Δ !! k) as [c0 | ] eqn:hc0.
+      - case : hc => <-.
+        apply SubConstraint.
+        apply elem_of_list_lookup_2 in hc0.
+        by destruct c0.
+      - apply list_lookup_fmap_inv in hc as [c1 [-> hc1]].
+        rewrite /subst_constraint /=.
+        inv hokt; simplify_eq.
+        by apply H4 in hc1.
+    }
+    iAssert (□ Σinterp (interp_list Σ (subst_ty σ <$> σt_o)) (constraints cdef))%I as "#hΣΔc".
+    { iModIntro.
+      iIntros (k c hc v) "hv".
+      inv hok0_; simplify_eq.
+      assert (hc' := hc).
+      apply H4 in hc'.
+      iDestruct ((subtype_is_inclusion _ hΔ wf_parent wf_mono wf_constraints_wf
+        wf_constraints_bounded _ _ _ _ hc') with "hΣ hΣΔ") as "hh"; try assumption.
+      { apply wf_ty_subst; first by apply wf_ty_subst_map.
+        apply wf_constraints_wf in hcdef.
+        rewrite /wf_cdef_constraints_wf Forall_lookup in hcdef.
+        by apply hcdef in hc as [].
+      }
+      assert (hbc: bounded_constraint (length (subst_ty σ <$> σt_o)) c).
+      { apply wf_constraints_bounded in hcdef.
+        rewrite /wf_cdef_constraints_bounded Forall_lookup in hcdef.
+        rewrite map_length -heq1.
+        by apply hcdef in hc.
+      }
+      destruct hbc as [].
+      rewrite interp_type_subst; last done.
+      rewrite interp_type_subst; last done.
+      by iApply "hh".
+    }
+    assert (hlc:
+      length (interp_list Σ (subst_ty σ <$> σt_o)) = length cdef.(generics)).
+    { by rewrite /interp_list !fmap_length heq1. }
+    assert (hentails_cdef: ∀ k s t,
+      cdef.(constraints) !! k = Some (s, t) → cdef.(constraints) ⊢ s <: t).
+    { move => ??? hc.
+      eapply SubConstraint.
+      by apply elem_of_list_lookup_2 in hc.
+    }
+    assert (hwfΔc: Forall wf_constraint cdef.(constraints)).
+    { by apply wf_constraints_wf in hcdef. }
+    assert (hbΔc: Forall (bounded_constraint (length cdef.(generics))) cdef.(constraints)).
+    { by apply wf_constraints_bounded in hcdef. }
+    iSpecialize ("IH" $! C _ Plain (length cdef.(generics)) _ _ _ hwf_lty0 hbounded hokc hwfΔc hbΔc
+    hbody (interp_list Σ (subst_ty σ <$> σt_o))  _ _ _ hlc heval_body with "hΣc hΣΔc"); simpl.
+    iDestruct ("IH" with "[Hh Hle H●]") as "Hstep".
+    { iClear "IH"; iSplit.
+      - iExists _; iFrame.
+        iSplit; last done.
+        by rewrite Hdom.
+      - iSplit => /=.
+        + iDestruct ((this_inherits_using_is_inclusion wf_parent Σ _ _ σ _ (LocV l) hin_t_o)) as "hh" => //.
+          destruct Γ as [[? ?] Γ].
+          destruct Ω as [vthis Ω].
+          rewrite /type_of_this in ht.
+          injection ht; intros; subst; clear ht.
+          iDestruct "Hle" as "[hthis _]".
+          simpl in heval_recv.
+          case: heval_recv => ->.
+          simpl.
+          iDestruct ("hh" with "hthis") as "hh2".
+          iClear "hΣ hΣΔ hthis Hl Hh HΦ H H▷ hh H●".
+          rewrite /interp_this_type.
+          rewrite interp_this_equivI; first done.
+          rewrite list_equiv_lookup => k.
+          rewrite !list_lookup_fmap.
+          destruct (decide (k < length cdef.(generics))) as [hlt | hge].
+          * assert (hh: is_Some (σt_o !! k)).
+            { rewrite heq1 in hlt.
+              by apply lookup_lt_is_Some_2 in hlt.
+            }
+            destruct hh as [ty hty]; rewrite hty /=.
+            rewrite lookup_seq_lt //=.
+            f_equiv => w.
+            by rewrite interp_generic_unfold /interp_generic /=
+              !list_lookup_fmap hty.
+          * assert (hle: length cdef.(generics) ≤ k) by lia.
+            rewrite lookup_seq_ge //=.
+            rewrite heq1 in hle.
+            by apply lookup_ge_None_2 in hle as ->.
+        + iIntros (v ty hv).
+          assert (ha: ∃ arg, args !! v = Some arg).
+          { apply elem_of_dom.
+            rewrite /subst_mdef /= !dom_fmap_L in hmdom.
+            rewrite -hdom /subst_mdef /= dom_fmap.
+            by apply elem_of_dom.
+          }
+          destruct ha as [arg ha].
+          assert (hvarg: ∃ varg, vargs !! v = Some varg).
+          { apply elem_of_dom.
+            apply dom_map_args in hmap.
+            rewrite hmap.
+            apply elem_of_dom.
+            now rewrite ha.
+          }
+          destruct hvarg as [varg hvarg].
+          iExists varg; rewrite hvarg; iSplitR; first done.
+          rewrite (map_args_lookup _ _ _ args vargs hmap v) ha /= in hvarg.
+          destruct (methodargs omdef !! v) as [tw | ] eqn:htw => //.
+          case: hv => <-; clear ty.
+          assert (h0: methodargs (subst_mdef σt_o omdef) !! v = Some (subst_ty σt_o tw)).
+          { by rewrite /subst_mdef /= !lookup_fmap htw. }
+          move: (hi v _ _ h0 ha) => haty.
+          iDestruct (expr_soundness with "hΣ hΣΔ Hle") as "he" => //.
+          assert (hb: bounded (length σt_o) tw).
+          { apply wf_methods_bounded in hcdef.
+            apply hcdef in homdef0.
+            apply homdef0 in htw.
+            by rewrite -heq1.
+          }
+          rewrite interp_type_subst; last by eapply bounded_subst.
+          rewrite interp_type_subst; last done.
+          rewrite interp_type_equivI; first done.
+          rewrite /interp_list -list_fmap_compose.
+          apply list_fmap_equiv_ext => k ty hty w /=.
+          rewrite interp_type_subst; first done.
+          apply inherits_using_wf in hin_t_o => //.
+          destruct hin_t_o as (? & ? & hB & ?); simplify_eq.
+          rewrite Forall_lookup in hB.
+          apply hB in hty.
+          inv hwfthis; simplify_eq.
+          by rewrite H4.
+    }
+    iRevert "Hstep".
+    iApply updN_mono_I.
+    iIntros "[Hmodels Hle2]"; iFrame.
+    iApply interp_local_tys_update; first by done.
+    assert (hb : bounded (length σt_o) (methodrettype omdef)).
+    { apply wf_methods_bounded in hcdef.
+      apply hcdef in homdef0.
+      rewrite -heq1.
+      by apply homdef0.
+    }
+    rewrite subst_ty_subst; last done.
+    rewrite interp_type_subst; last by rewrite map_length.
+    by iApply (expr_soundness _ _ (interp_list Σ (subst_ty σ <$> σt_o)) _ _ Γ').
+  Qed.
+End proofs.
