theories/soundness/rtc_tag.v
@@ -30,6 +30,7 @@ Section proofs.
     wf_cdefs pdefs →
     wf_lty Γ0 →
     bounded_lty rigid Γ0 →
+    ok_ty Δ (this_type Γ0) →
     Forall wf_constraint Δ →
     Forall (bounded_constraint rigid) Δ →
     ctxt Γ0 !! v = Some tv →
@@ -45,43 +46,56 @@ Section proofs.
     cmd_eval C st (RuntimeCheckC v (RCTag t) thn els) st' n →
     □ interp_env_as_mixed Σ -∗
     □ Σinterp Σ Δ -∗
-    □ (⌜wf_lty
-          (<[v:=InterT tv
-               (ClassT t (map GenT (seq rigid (length (generics def)))))]>
-               Γ0)⌝ →
-       ⌜bounded_lty (rigid + length (generics def))
-             (<[v:=InterT tv
-                   (ClassT t
-                      (map GenT (seq rigid (length (generics def)))))]> Γ0)⌝ →
-       ⌜Forall wf_constraint (lift_constraints rigid (constraints def) ++ Δ)⌝ →
-       ⌜Forall (bounded_constraint (rigid + length (generics def)))
-               (lift_constraints rigid (constraints def) ++ Δ)⌝ →
-       ∀ (a : list (interp Θ)) (a0 a1 : local_env * heap) (a2 : nat),
-         ⌜length a = (rigid + length (generics def))%nat⌝ -∗
-         ⌜cmd_eval C a0 thn a1 a2⌝ -∗
-         □ interp_env_as_mixed a -∗
-         □ Σinterp a (lift_constraints rigid (constraints def) ++ Δ) -∗
-         heap_models a0.2 ∗
-            interp_local_tys a
-                     (<[v:=InterT tv
-                           (ClassT t (map GenT (seq rigid (length (generics def)))))]>
-                        Γ0) a0.1 -∗
-         |=▷^a2 heap_models a1.2 ∗ interp_local_tys a Γ1 a1.1) -∗
-    □ (⌜wf_lty Γ0⌝ →
-       ⌜bounded_lty rigid Γ0⌝ →
-       ⌜Forall wf_constraint Δ⌝ →
-       ⌜Forall (bounded_constraint rigid) Δ⌝ →
-       ∀ (a : list (interp Θ)) (a0 a1 : local_env * heap) (a2 : nat),
-         ⌜length a = rigid⌝ -∗
-         ⌜cmd_eval C a0 els a1 a2⌝ -∗
-         □ interp_env_as_mixed a -∗
-         □ Σinterp a Δ -∗
-         heap_models a0.2 ∗ interp_local_tys a Γ0 a0.1 -∗
-     |=▷^a2 heap_models a1.2 ∗ interp_local_tys a Γ1 a1.1) -∗
+    □ ( ⌜wf_lty
+            (<[v:=InterT tv
+                    (ClassT t (map GenT (seq rigid (length (generics def)))))]>
+               Γ0)⌝
+         → ⌜bounded_lty (rigid + length (generics def))
+              (<[v:=InterT tv
+                      (ClassT t
+                         (map GenT (seq rigid (length (generics def)))))]> Γ0)⌝
+           → ⌜ok_ty (lift_constraints rigid (constraints def) ++ Δ)
+                (this_type
+                   (<[v:=InterT tv
+                           (ClassT t
+                              (map GenT (seq rigid (length (generics def)))))]>
+                      Γ0))⌝
+             → ⌜Forall wf_constraint
+                  (lift_constraints rigid (constraints def) ++ Δ)⌝
+               → ⌜Forall (bounded_constraint (rigid + length (generics def)))
+                    (lift_constraints rigid (constraints def) ++ Δ)⌝
+                 → ∀ (a : list (interp Θ)) (a0 a1 : local_env * heap)
+                     (a2 : nat),
+                     ⌜length a = (rigid + length (generics def))%nat⌝ -∗
+                     ⌜cmd_eval C a0 thn a1 a2⌝ -∗
+                     □ interp_env_as_mixed a -∗
+                     □ Σinterp a
+                         (lift_constraints rigid (constraints def) ++ Δ) -∗
+                     heap_models a0.2 ∗
+                     interp_local_tys a
+                       (<[v:=InterT tv
+                               (ClassT t
+                                  (map GenT
+                                     (seq rigid (length (generics def)))))]>
+                          Γ0) a0.1 -∗
+                     |=▷^a2 heap_models a1.2 ∗ interp_local_tys a Γ1 a1.1) -∗
+    □ ( ⌜wf_lty Γ0⌝
+          → ⌜bounded_lty rigid Γ0⌝
+            → ⌜ok_ty Δ (this_type Γ0)⌝
+              → ⌜Forall wf_constraint Δ⌝
+                → ⌜Forall (bounded_constraint rigid) Δ⌝
+                  → ∀ (a : list (interp Θ)) (a0 a1 : local_env * heap)
+                      (a2 : nat),
+                      ⌜length a = rigid⌝ -∗
+                      ⌜cmd_eval C a0 els a1 a2⌝ -∗
+                      □ interp_env_as_mixed a -∗
+                      □ Σinterp a Δ -∗
+                      heap_models a0.2 ∗ interp_local_tys a Γ0 a0.1 -∗
+                      |=▷^a2 heap_models a1.2 ∗ interp_local_tys a Γ1 a1.1) -∗
      heap_models st.2 ∗ interp_local_tys Σ Γ0 st.1 -∗
      |=▷^n heap_models st'.2 ∗ interp_local_tys Σ Γ1 st'.1.
   Proof.
-    move => wfpdefs wflty blty ? hΔb hv hdef hthn hels Σ st st' n hrigid hc.
+    move => wfpdefs wflty blty hokthis ? hΔb hv hdef hthn hels Σ st st' n hrigid hc.
     iIntros "#hΣ #hΣΔ #Hthn #Hels".
     inv hc; last first.
     { iIntros "[Hh H]".
@@ -259,6 +273,10 @@ Section proofs.
       { iApply "Hthn".
         - by iPureIntro.
         - by iPureIntro.
+        - iPureIntro; move: hokthis.
+          destruct Γ0 as [[this σ] Γ0]; rewrite /this_type /= => hok.
+          eapply ok_ty_weaken; first by apply hok.
+          by set_solver.
         - iPureIntro.
           apply Forall_app; split.
           + apply lift_constraints_wf.
